Kraken.lean
@@ -26,4 +26,5 @@ import Kraken.Easm
 import Kraken.MachineWP
 import Kraken.SepWP
 import Kraken.SepSpecs
+import Kraken.SepFrameProc
 import Kraken.X64.Examples.AluMemSep
